books/branches/jared/centaur/esim/stv/stv2c/alu16.cc
@@ -1,0 +1,352 @@
+// ESIM Symbolic Hardware Simulator
+// Copyright (C) 2010-2012 Centaur Technology
+//
+// Contact:
+//   Centaur Technology Formal Verification Group
+//   7600-C N. Capital of Texas Highway, Suite 300, Austin, TX 78731, USA.
+//   http://www.centtech.com/
+//
+// This program is free software; you can redistribute it and/or modify it under
+// the terms of the GNU General Public License as published by the Free Software
+// Foundation; either version 2 of the License, or (at your option) any later
+// version.  This program is distributed in the hope that it will be useful but
+// WITHOUT ANY WARRANTY; without even the implied warranty of MERCHANTABILITY or
+// FITNESS FOR A PARTICULAR PURPOSE.  See the GNU General Public License for
+// more details.  You should have received a copy of the GNU General Public
+// License along with this program; if not, write to the Free Software
+// Foundation, Inc., 51 Franklin Street, Suite 500, Boston, MA 02110-1335, USA.
+//
+// alu16.cc -- Test bench of the C++ code for the alu16 module
+//
+// Original author: Jared Davis <jared@centtech.com>
+
+#include "alu16_test.h"
+#include <iostream>
+using namespace std;
+
+#define VERBOSE 0
+
+// This is a test bench to see if our C++ translation of alu16.v seems to be
+// correct.  I don't bother to test the COUNT operation because it has a "bug"
+// that I don't want to reimplement.
+
+static const uint8_t OP_PLUS = 0;
+static const uint8_t OP_MINUS = 1;
+static const uint8_t OP_BITAND = 2;
+static const uint8_t OP_BITOR = 3;
+static const uint8_t OP_BITXOR = 4;
+static const uint8_t OP_MIN = 5;
+static const uint8_t OP_COUNT = 6;
+static const uint8_t OP_MULT = 7;
+
+bool check_all(const fourval<16>& a, const fourval<16>& b);
+
+fourval<16> plus_spec(const fourval<16>& a, const fourval<16>& b);
+fourval<16> minus_spec(const fourval<16>& a, const fourval<16>& b);
+fourval<16> bitand_spec(const fourval<16>& a, const fourval<16>& b);
+fourval<16> bitor_spec(const fourval<16>& a, const fourval<16>& b);
+fourval<16> bitxor_spec(const fourval<16>& a, const fourval<16>& b);
+fourval<16> min_spec(const fourval<16>& a, const fourval<16>& b);
+fourval<16> mult_spec(const fourval<16>& a, const fourval<16>& b);
+
+int main()
+{
+    bool ok = true;
+
+    uint16_t stop = VERBOSE ? 100 : 10000;
+
+    cout << "-- Pure Boolean checks --" << endl;
+    for(uint16_t i = 0; i < stop; ++i)
+    {
+	if (VERBOSE) { cout << endl; }
+	uint16_t rand1 = rand();
+	uint16_t rand2 = rand();
+	fourval<16> a = fourval<16>(rand1);
+	fourval<16> b = fourval<16>(rand2);
+	if (VERBOSE) { cout << "A is " << a << endl; }
+	if (VERBOSE) { cout << "B is " << b << endl; }
+	ok &= check_all(a,b);
+    }
+
+    cout << "-- Pure random onset/offset checks --" << endl;
+    for(uint16_t i = 0; i < stop; ++i)
+    {
+	if (VERBOSE) { cout << endl; }
+	uint16_t rand1 = rand();
+	uint16_t rand2 = rand();
+	uint16_t rand3 = rand();
+	uint16_t rand4 = rand();
+	fourval<16> a = fourval<16>(rand1, rand2);
+	fourval<16> b = fourval<16>(rand3, rand4);
+	if (VERBOSE) { cout << "A is " << a << endl; }
+	if (VERBOSE) { cout << "B is " << b << endl; }
+	ok &= check_all(a,b);
+    }
+
+    cout << "-- Almost pure-Boolean checks. --" << endl;
+    for(uint16_t i = 0; i < stop; ++i)
+    {
+	if (VERBOSE) { cout << endl; }
+	uint16_t rand1 = rand();
+	uint16_t rand2 = rand();
+	fourval<16> a = fourval<16>(rand1);
+	fourval<16> b = fourval<16>(rand2);
+	if (i % 2) {
+	    uint16_t place = i % 16;
+	    b.onset.cpyBit(place, b.offset.getBit(place));
+	}
+	else {
+	    uint16_t place = i % 16;
+	    b.offset.cpyBit(place, b.onset.getBit(place));
+	}
+	if (VERBOSE) { cout << "A is " << a << endl; }
+	if (VERBOSE) { cout << "B is " << b << endl; }
+	ok &= check_all(a,b);
+    }
+
+    if (ok) {
+	cout << "Checks passed." << endl;
+	exit(0);
+    }
+    else {
+	cout << "Checks failed." << endl;
+	exit(1);
+    }
+}
+
+bool check_all(const fourval<16>& a, const fourval<16>& b)
+{
+    bool ok = true;
+
+    alu16_test_ins in;
+    alu16_test_outs out;
+    fourval<16> spec;
+    in.a = a;
+    in.b = b;
+
+    in.op = fourval<3>(OP_PLUS);
+    alu16_test_run(in, out);
+    spec = plus_spec(a,b);
+    if (VERBOSE) { cout << "+    " << out.res << endl; }
+    if (out.res != spec) {
+	cout << "Mismatch for plus(" << a << ", " << b << "): "
+	     << out.res << " vs. " << spec << endl;
+	ok = false;
+    }
+
+    in.op = fourval<3>(OP_MINUS);
+    alu16_test_run(in, out);
+    spec = minus_spec(a,b);
+    if (VERBOSE) { cout << "-    " << out.res << endl; }
+    if (out.res != spec) {
+	cout << "Mismatch for minus(" << a << ", " << b << "): "
+	     << out.res << " vs. " << spec << endl;
+	ok = false;
+    }
+
+    in.op = fourval<3>(OP_BITAND);
+    alu16_test_run(in, out);
+    spec = bitand_spec(a,b);
+    if (VERBOSE) { cout << "&    " << out.res << endl; }
+    if (out.res != spec) {
+	cout << "Mismatch for bitand(" << a << ", " << b << "): "
+	     << out.res << " vs. " << spec << endl;
+	ok = false;
+    }
+
+    in.op = fourval<3>(OP_BITOR);
+    alu16_test_run(in, out);
+    spec = bitor_spec(a,b);
+    if (VERBOSE) { cout << "|    " << out.res << endl; }
+    if (out.res != spec) {
+	cout << "Mismatch for bitor(" << a << ", " << b << "): "
+	     << out.res << " vs. " << spec << endl;
+	ok = false;
+    }
+
+    in.op = fourval<3>(OP_BITXOR);
+    alu16_test_run(in, out);
+    spec = bitxor_spec(a,b);
+    if (VERBOSE) { cout << "^    " << out.res << endl; }
+    if (out.res != spec) {
+	cout << "Mismatch for bitxor(" << a << ", " << b << "): "
+	     << out.res << " vs. " << spec << endl;
+	ok = false;
+    }
+
+    in.op = fourval<3>(OP_MIN);
+    alu16_test_run(in, out);
+    spec = min_spec(a,b);
+    if (VERBOSE) { cout << "^    " << out.res << endl; }
+    if (out.res != spec) {
+	cout << "Mismatch for min(" << a << ", " << b << "): "
+	     << out.res << " vs. " << spec << endl;
+	ok = false;
+    }
+
+    in.op = fourval<3>(OP_MULT);
+    alu16_test_run(in, out);
+    spec = mult_spec(a,b);
+    if (VERBOSE) { cout << "*    " << out.res << endl; }
+    if (out.res != mult_spec(a,b)) {
+	cout << "Mismatch for mult(" << a << ", " << b << "): "
+	     << out.res << " vs. " << spec << endl;
+	ok = false;
+    }
+
+    return ok;
+}
+
+fourval<16> plus_spec(const fourval<16>& a, const fourval<16>& b)
+{
+    if (a.isPureBoolean() && b.isPureBoolean())
+    {
+	const bit<16>& aval = a.onset;
+	const bit<16>& bval = b.onset;
+	const bit<16> ans = aval + bval;
+	return fourval<16>(ans);
+    }
+    else
+    {
+	return fourval<16>::all_X();
+    }
+}
+
+fourval<16> minus_spec(const fourval<16>& a, const fourval<16>& b)
+{
+    if (a.isPureBoolean() && b.isPureBoolean())
+    {
+	const bit<16>& aval = a.onset;
+	const bit<16>& bval = b.onset;
+	const bit<16> ans = aval - bval;
+	return fourval<16>(ans);
+    }
+    else
+    {
+	return fourval<16>::all_X();
+    }
+}
+
+fourval<16> bitand_spec(const fourval<16>& a, const fourval<16>& b)
+{
+    fourval<16> ans;
+    for(int i = 0;i < 16;++i) {
+	bool a1 = a.onset.getBit(i);
+	bool a0 = a.offset.getBit(i);
+	bool b1 = b.onset.getBit(i);
+	bool b0 = b.offset.getBit(i);
+	bool ans1;
+	bool ans0;
+	if (!a1 && a0) { // A is false, so it's false
+	    ans1 = false;
+	    ans0 = true;
+	}
+	else if (!b1 && b0) { // B is false, so it's false
+	    ans1 = false;
+	    ans0 = true;
+	}
+	else if (a1 && !a0 && b1 && !b0) { // Both are 1, so it's true
+	    ans1 = true;
+	    ans0 = false;
+	}
+	else { // else X
+	    ans1 = true;
+	    ans0 = true;
+	}
+	ans.onset.cpyBit(i, ans1);
+	ans.offset.cpyBit(i, ans0);
+    }
+    return ans;
+}
+
+fourval<16> bitor_spec(const fourval<16>& a, const fourval<16>& b)
+{
+    fourval<16> ans;
+    for(int i = 0;i < 16;++i) {
+	bool a1 = a.onset.getBit(i);
+	bool a0 = a.offset.getBit(i);
+	bool b1 = b.onset.getBit(i);
+	bool b0 = b.offset.getBit(i);
+	bool ans1;
+	bool ans0;
+	if (a1 && !a0) { // A is true, so it's true
+	    ans1 = true;
+	    ans0 = false;
+	}
+	else if (b1 && !b0) { // B is true, so it's true
+	    ans1 = true;
+	    ans0 = false;
+	}
+	else if (!a1 && a0 && !b1 && b0) { // Both are 0, so it's false
+	    ans1 = false;
+	    ans0 = true;
+	}
+	else { // else X
+	    ans1 = true;
+	    ans0 = true;
+	}
+	ans.onset.cpyBit(i, ans1);
+	ans.offset.cpyBit(i, ans0);
+    }
+    return ans;
+}
+
+fourval<16> bitxor_spec(const fourval<16>& a, const fourval<16>& b)
+{
+    fourval<16> ans;
+    for(int i = 0;i < 16;++i) {
+	bool a1 = a.onset.getBit(i);
+	bool a0 = a.offset.getBit(i);
+	bool b1 = b.onset.getBit(i);
+	bool b0 = b.offset.getBit(i);
+	bool ans1;
+	bool ans0;
+	if (a1 != a0 && b1 != b0) { // Good boolean values
+	    ans1 = a1 != b1;
+	    ans0 = a1 == b1;
+	}
+	else { // Anything else is X.
+	    ans1 = true;
+	    ans0 = true;
+	}
+	ans.onset.cpyBit(i, ans1);
+	ans.offset.cpyBit(i, ans0);
+    }
+    return ans;
+}
+
+fourval<16> min_spec(const fourval<16>& a, const fourval<16>& b)
+{
+    // The alu16.v definition is (abus < bbus) ? abus : bbus.  Per Verilog
+    // semantics, the comparison operator yields X if either operand has any X
+    // bit.  In that case, the ?: operator semantics are that we merge any bits
+    // that agree on good Boolean values.  But VL uses (by default) a more
+    // conservative semantics, where X ? a : b always returns Xes.
+
+    if (a.isPureBoolean() && b.isPureBoolean())
+    {
+	const bit<16>& aval = a.onset;
+	const bit<16>& bval = b.onset;
+	const bit<16> ans = aval < bval ? aval : bval;
+	return fourval<16>(ans);
+    }
+    else
+    {
+	return fourval<16>::all_X();
+    }
+}
+
+fourval<16> mult_spec(const fourval<16>& a, const fourval<16>& b)
+{
+    if (a.isPureBoolean() && b.isPureBoolean())
+    {
+	uint16_t aval = (uint16_t)a.onset;
+	uint16_t bval = (uint16_t)b.onset;
+	uint16_t ans = aval * bval;
+	return fourval<16>(ans);
+    }
+    else
+    {
+	return fourval<16>::all_X();
+    }
+}
