books/branches/jared/centaur/esim/stv/stv2c/fourval.h
@@ -1,0 +1,128 @@
+// ESIM Symbolic Hardware Simulator
+// Copyright (C) 2010-2013 Centaur Technology
+//
+// Contact:
+//   Centaur Technology Formal Verification Group
+//   7600-C N. Capital of Texas Highway, Suite 300, Austin, TX 78731, USA.
+//   http://www.centtech.com/
+//
+// This program is free software; you can redistribute it and/or modify it under
+// the terms of the GNU General Public License as published by the Free Software
+// Foundation; either version 2 of the License, or (at your option) any later
+// version.  This program is distributed in the hope that it will be useful but
+// WITHOUT ANY WARRANTY; without even the implied warranty of MERCHANTABILITY or
+// FITNESS FOR A PARTICULAR PURPOSE.  See the GNU General Public License for
+// more details.  You should have received a copy of the GNU General Public
+// License along with this program; if not, write to the Free Software
+// Foundation, Inc., 51 Franklin Street, Suite 500, Boston, MA 02110-1335, USA.
+//
+// fourval.h -- Arbitrary (but fixed) width four-valued integer type
+//
+// Original authors: Nikhil Patil <npatil@centtech.com>
+//                   Jared Davis <jared@centtech.com>
+
+#pragma once
+#include "bits.h"
+#include <iostream>
+
+// We use a simple onset/offset encoding:
+//
+//   ONSET    OFFSET     VALUE
+// -------------------------------
+//     1        1          X
+//     1        0          1
+//     0        1          0
+//     0        0          Z
+// -------------------------------
+
+template <unsigned N>
+class fourval {
+public:
+
+    bit<N> onset;
+    bit<N> offset;
+
+    // Default constructor initializes the value to all good, Boolean zeros.
+    fourval<N>()
+	: onset(bit<N>::zero()),
+	  offset(~bit<N>::zero())
+    {}
+
+    // Promotion from bit<N> into a pure Boolean fourval<N>
+    explicit fourval<N>(bit<N> on)
+	: onset(on),
+	  offset(~on)
+    {}
+
+    // Explicit construction of fourval<N> with control over onset/offset
+    explicit fourval<N>(bit<N> on, bit<N> off)
+      : onset(on),
+        offset(off)
+    {}
+
+
+    // Some useful fourval<N> constructors for all 0s, 1s, Xes, Zs.
+
+    static fourval<N> all_0() {
+	return fourval<N>(bit<N>::zero(), ~bit<N>::zero());
+    }
+
+    static fourval<N> all_1() {
+	return fourval<N>(~bit<N>::zero(), bit<N>::zero());
+    }
+
+    static fourval<N> all_X() {
+	return fourval<N>(~bit<N>::zero(), ~bit<N>::zero());
+    }
+
+    static fourval<N> all_Z() {
+	return fourval<N>(bit<N>::zero(), bit<N>::zero());
+    }
+
+
+    bool isPureBoolean() const {
+	// Returns true iff every bit is 1 or 0---that is, if no bit
+	// anywhere is ever X or Z.
+	return onset == ~offset;
+    }
+
+    bit<N> pureBooleanMask() const {
+	// Returns an N-bit mask, where mask[i] == 1 exactly when the ith
+	// bit is Boolean-valued, i.e., not X or Z.
+	return onset ^ offset;
+    }
+
+
+    // Some basic operators.  BOZO, it would probably be convenient to
+    // have many additional operators, e.g., +, -, *, &, etc., perhaps
+    // with Verilog semantics for X handling.
+
+    bool operator ==(const fourval<N> &that) const {
+	return onset == that.onset
+    	    && offset == that.offset;
+    }
+
+    bool operator !=(const fourval<N> &that) const {
+        return !(*this == that);
+    }
+};
+
+template<unsigned N>
+std::ostream& operator<< (std::ostream& stream, const fourval<N>& x)
+{
+    stream << N << "'b";
+    unsigned i = N;
+    while(i)
+    {
+	--i;
+	bool on = x.onset.getBit(i);
+	bool off = x.offset.getBit(i);
+	char c = (on && off) ? 'X'
+	       : (on && !off) ? '1'
+	       : (!on && off) ? '0'
+	       : 'Z';
+	stream << c;
+    }
+    return stream;
+}
+
