books/branches/jared/centaur/esim/stv/stv2c/test_bits.cc
@@ -1,0 +1,217 @@
+// ESIM Symbolic Hardware Simulator
+// Copyright (C) 2010-2012 Centaur Technology
+//
+// Contact:
+//   Centaur Technology Formal Verification Group
+//   7600-C N. Capital of Texas Highway, Suite 300, Austin, TX 78731, USA.
+//   http://www.centtech.com/
+//
+// This program is free software; you can redistribute it and/or modify it under
+// the terms of the GNU General Public License as published by the Free Software
+// Foundation; either version 2 of the License, or (at your option) any later
+// version.  This program is distributed in the hope that it will be useful but
+// WITHOUT ANY WARRANTY; without even the implied warranty of MERCHANTABILITY or
+// FITNESS FOR A PARTICULAR PURPOSE.  See the GNU General Public License for
+// more details.  You should have received a copy of the GNU General Public
+// License along with this program; if not, write to the Free Software
+// Foundation, Inc., 51 Franklin Street, Suite 500, Boston, MA 02110-1335, USA.
+//
+// test_bits.cc -- Tests of bit<n> datatype
+//
+// Original authors: Nikhil Patil <npatil@centtech.com>
+//                   Jared Davis <jared@centtech.com>
+
+#include "bits.h"
+#include "fourval.h"
+#include <iostream>
+#include <cstdlib>
+
+using namespace std;
+
+void test_bit_twiddling();
+void test_four_valued();
+
+int main()
+{
+    auto val = bit<666>::zero();
+    val.setBit(109).setBit(9).setBit(8);
+    printf("%d %d %d\n", val.getBit(9), val.getBit(8), val.getBit(109));
+
+    test_bit_twiddling();
+    test_four_valued();
+}
+
+void test_bit_twiddling()
+{
+    auto x1 = bit<1>::zero();
+    assert(x1.getBit(0) == false);
+    x1.setBit(0);
+    assert(x1.getBit(0) == true);
+    x1.clrBit(0);
+    assert(x1.getBit(0) == false);
+    x1.cpyBit(0, true);
+    assert(x1.getBit(0) == true);
+    x1.cpyBit(0, false);
+    assert(x1.getBit(0) == false);
+
+    auto x2 = bit<2>::zero();
+    assert(x2.getBit(0) == false);
+    assert(x2.getBit(1) == false);
+    x2.setBit(0);
+    assert(x2.getBit(0) == true);
+    assert(x2.getBit(1) == false);
+    x2.clrBit(0);
+    assert(x2.getBit(0) == false);
+    assert(x2.getBit(1) == false);
+    x2.cpyBit(0, true);
+    assert(x2.getBit(0) == true);
+    assert(x2.getBit(1) == false);
+    x2.cpyBit(0, false);
+    assert(x2.getBit(0) == false);
+    assert(x2.getBit(1) == false);
+    x2.setBit(1);
+    assert(x2.getBit(0) == false);
+    assert(x2.getBit(1) == true);
+    x2.clrBit(1);
+    assert(x2.getBit(0) == false);
+    assert(x2.getBit(1) == false);
+    x2.cpyBit(1, true);
+    assert(x2.getBit(0) == false);
+    assert(x2.getBit(1) == true);
+    x2.cpyBit(1, false);
+    assert(x2.getBit(0) == false);
+    assert(x2.getBit(1) == false);
+
+    auto x8 = bit<8>::zero();
+    assert(x8.getBit(0) == false);
+    assert(x8.getBit(7) == false);
+    x8.setBit(0);
+    assert(x8.getBit(0) == true);
+    assert(x8.getBit(7) == false);
+    x8.clrBit(0);
+    assert(x8.getBit(0) == false);
+    assert(x8.getBit(7) == false);
+    x8.cpyBit(0, true);
+    assert(x8.getBit(0) == true);
+    assert(x8.getBit(7) == false);
+    x8.cpyBit(0, false);
+    assert(x8.getBit(0) == false);
+    assert(x8.getBit(7) == false);
+    x8.setBit(7);
+    assert(x8.getBit(0) == false);
+    assert(x8.getBit(7) == true);
+    x8.clrBit(7);
+    assert(x8.getBit(0) == false);
+    assert(x8.getBit(7) == false);
+    x8.cpyBit(7, true);
+    assert(x8.getBit(0) == false);
+    assert(x8.getBit(7) == true);
+    x8.cpyBit(7, false);
+    assert(x8.getBit(0) == false);
+    assert(x8.getBit(7) == false);
+
+    auto x3 = bit<19>::zero();
+    assert(x3.getBit(0) == false);
+    assert(x3.getBit(17) == false);
+    x3.setBit(0);
+    assert(x3.getBit(0) == true);
+    assert(x3.getBit(17) == false);
+    x3.clrBit(0);
+    assert(x3.getBit(0) == false);
+    assert(x3.getBit(17) == false);
+    x3.cpyBit(0, true);
+    assert(x3.getBit(0) == true);
+    assert(x3.getBit(17) == false);
+    x3.cpyBit(0, false);
+    assert(x3.getBit(0) == false);
+    assert(x3.getBit(17) == false);
+    x3.setBit(17);
+    assert(x3.getBit(0) == false);
+    assert(x3.getBit(17) == true);
+    x3.clrBit(17);
+    assert(x3.getBit(0) == false);
+    assert(x3.getBit(17) == false);
+    x3.cpyBit(17, true);
+    assert(x3.getBit(0) == false);
+    assert(x3.getBit(17) == true);
+    x3.cpyBit(17, false);
+    assert(x3.getBit(0) == false);
+    assert(x3.getBit(17) == false);
+
+
+    auto x4 = bit<203>::zero();
+    assert(x4.getBit(0) == false);
+    assert(x4.getBit(155) == false);
+    x4.setBit(0);
+    assert(x4.getBit(0) == true);
+    assert(x4.getBit(155) == false);
+    x4.clrBit(0);
+    assert(x4.getBit(0) == false);
+    assert(x4.getBit(155) == false);
+    x4.cpyBit(0, true);
+    assert(x4.getBit(0) == true);
+    assert(x4.getBit(155) == false);
+    x4.cpyBit(0, false);
+    assert(x4.getBit(0) == false);
+    assert(x4.getBit(155) == false);
+    x4.setBit(155);
+    assert(x4.getBit(0) == false);
+    assert(x4.getBit(155) == true);
+    x4.clrBit(155);
+    assert(x4.getBit(0) == false);
+    assert(x4.getBit(155) == false);
+    x4.cpyBit(155, true);
+    assert(x4.getBit(0) == false);
+    assert(x4.getBit(155) == true);
+    x4.cpyBit(155, false);
+    assert(x4.getBit(0) == false);
+    assert(x4.getBit(155) == false);
+}
+
+
+void test_four_valued()
+{
+    auto x1 = fourval<1>::all_0();
+    assert(x1.onset.getBit(0) == false);
+    assert(x1.offset.getBit(0) == true);
+    assert(x1.isPureBoolean());
+    cout << x1 << endl;
+
+    auto x2 = fourval<2>::all_0();
+    assert(x2.onset.getBit(0) == false);
+    assert(x2.offset.getBit(0) == true);
+    assert(x2.isPureBoolean());
+    cout << x2 << endl;
+
+    auto x3 = fourval<20>::all_0();
+    assert(x3.onset.getBit(0) == false);
+    assert(x3.offset.getBit(0) == true);
+    assert(x3.isPureBoolean());
+    cout << x3 << endl;
+
+    auto x4 = fourval<23>::all_0();
+    assert(x4.onset.getBit(0) == false);
+    assert(x4.offset.getBit(0) == true);
+    assert(x4.isPureBoolean());
+    cout << "all zeros: " << x4 << endl;
+
+    auto x5 = fourval<23>::all_1();
+    assert(x5.onset.getBit(0) == true);
+    assert(x5.offset.getBit(0) == false);
+    assert(x5.isPureBoolean());
+    cout << "all ones: " << x5 << endl;
+
+    auto x6 = fourval<23>::all_X();
+    assert(x6.onset.getBit(0) == true);
+    assert(x6.offset.getBit(0) == true);
+    assert(!x6.isPureBoolean());
+    cout << "all xes: " << x6 << endl;
+
+    auto x7 = fourval<23>::all_Z();
+    assert(x7.onset.getBit(0) == false);
+    assert(x7.offset.getBit(0) == false);
+    assert(!x7.isPureBoolean());
+    cout << "all zes: " << x7 << endl;
+
+
+}
