books/branches/jared/centaur/aignet/aiger.lisp
@@ -1,0 +1,1159 @@
+; AIGNET - And-Inverter Graph Networks
+; Copyright (C) 2013 Centaur Technology
+;
+; Contact:
+;   Centaur Technology Formal Verification Group
+;   7600-C N. Capital of Texas Highway, Suite 300, Austin, TX 78731, USA.
+;   http://www.centtech.com/
+;
+; This program is free software; you can redistribute it and/or modify it under
+; the terms of the GNU General Public License as published by the Free Software
+; Foundation; either version 2 of the License, or (at your option) any later
+; version.  This program is distributed in the hope that it will be useful but
+; WITHOUT ANY WARRANTY; without even the implied warranty of MERCHANTABILITY or
+; FITNESS FOR A PARTICULAR PURPOSE.  See the GNU General Public License for
+; more details.  You should have received a copy of the GNU General Public
+; License along with this program; if not, write to the Free Software
+; Foundation, Inc., 51 Franklin Street, Suite 500, Boston, MA 02110-1335, USA.
+;
+; Original author: Sol Swords <sswords@centtech.com>
+
+(in-package "AIGNET")
+(include-book "from-hons-aig")
+(include-book "centaur/aig/aiger" :dir :system)
+(include-book "tools/defmacfun" :dir :system)
+(local (include-book "clause-processors/instantiate" :dir :system))
+(local (include-book "arithmetic/top-with-meta" :dir :system))
+(set-state-ok t)
+
+(local (in-theory (disable acl2::nth-with-large-index
+                           nth update-nth
+                           state-p1-forward)))
+(local (in-theory (enable* acl2::arith-equiv-forwarding)))
+
+(defstobj-clone aigernums u32arr :suffix "-AIGER")
+
+(local (in-theory (disable acl2::update-nth-update-nth)))
+
+
+(defsection aignet-aiger-number-nodes
+  ;; Assign each node its aiger ID and record it in aigernums.  Regoffset is
+  ;; 1+ninputs, which is added to the IO num of each register to make its aiger
+  ;; ID.  An input's ID is made by adding 1 to its IO num.  Gates are numbered
+  ;; sequentially, tracked by nextgate, which starts at 1+nins+nregs.
+  (defiteration aignet-aiger-number-nodes (aignet aigernums)
+    (declare (xargs :stobjs (aignet aigernums)
+                    :guard (<= (num-nodes aignet) (u32-length aigernums))
+                    :guard-hints (("goal" :in-theory (enable aignet-idp)))))
+    (b* ((type (id->type n aignet))
+         (nextgate (lnfix nextgate))
+         ((when (int= type (out-type)))
+          (mv aigernums nextgate))
+         (val (aignet-seq-case
+               type (io-id->regp n aignet)
+               :gate  nextgate
+               :pi    (+ 1 (io-id->ionum n aignet))
+               :reg   (+ 1 (num-ins aignet) (io-id->ionum n aignet))
+               :const 0))
+         (nextgate (if (int= type (gate-type))
+                       (1+ nextgate)
+                     nextgate))
+         (aigernums (set-u32 n val aigernums)))
+      (mv aigernums nextgate))
+    :returns (mv aigernums nextgate)
+    :top-returns aigernums
+    :index n
+    :init-vals ((nextgate (+ 1 (num-ins aignet) (num-regs aignet))))
+    :iter-decls ((type (integer 0 *) nextgate))
+    :first 0
+    :last (num-nodes aignet))
+
+  (in-theory (disable aignet-aiger-number-nodes))
+  (local (in-theory (enable aignet-aiger-number-nodes)))
+
+  (defthm natp-of-aignet-aiger-number-nodes-iter-nextgate
+    (implies (natp nextgate)
+             (natp (mv-nth 1 (aignet-aiger-number-nodes-iter n nextgate aignet aigernums))))
+    :hints((acl2::just-induct-and-expand
+            (aignet-aiger-number-nodes-iter n nextgate aignet aigernums)))
+    :rule-classes :type-prescription)
+
+  ;; (defun aignet-aiger-number-nodes-iter (n regoffset nextgate aignet aigernums)
+  ;;   (declare (type (integer 0 *) n)
+  ;;            (type (integer 0 *) regoffset)
+  ;;            (type (integer 0 *) nextgate)
+  ;;            (xargs :stobjs (aignet aigernums)
+  ;;                   :guard (and (u32arr-sizedp aigernums aignet)
+  ;;                               (aignet-iterator-p n aignet))
+  ;;                   :measure (nfix (- (nfix (num-nodes aignet)) (nfix n)))))
+  ;;   (b* (((when (mbe :logic (zp (- (nfix (num-nodes aignet)) (nfix n)))
+  ;;                    :exec (int= (num-nodes aignet) n)))
+  ;;         aigernums)
+  ;;        (nextgate (lnfix nextgate))
+  ;;        ((mv aigernums nextgate)
+  ;;         (case (id->type (to-id n) aignet)
+  ;;           (1 ;; gate
+  ;;            (b* ((aigernums (set-u32 n nextgate aigernums)))
+  ;;              (mv aigernums (1+ nextgate))))
+  ;;           (2 ;; CI
+  ;;            (b* ((aigernums (set-u32 n (+ (if (int= (io-id->regp (to-id n) aignet) 1)
+  ;;                                              (lnfix regoffset)
+  ;;                                            1)
+  ;;                                          (io-id->ionum (to-id n) aignet))
+  ;;                                     aigernums)))
+  ;;              (mv aigernums nextgate)))
+  ;;           (3 ;; CO -- skip
+  ;;            (mv aigernums nextgate))
+  ;;           (otherwise ;; 0 -- const
+  ;;            (b* ((aigernums (set-u32 n 0 aigernums)))
+  ;;              (mv aigernums nextgate))))))
+  ;;     (aignet-aiger-number-nodes-iter (1+ (lnfix n)) regoffset nextgate aignet
+  ;;                               aigernums)))
+
+  (defthm aigernums-size-of-aignet-aiger-number-nodes-iter
+    (implies (< (node-count aignet) (len aigernums))
+             (< (node-count aignet) (len (mv-nth 0 (aignet-aiger-number-nodes-iter
+                                                    n nextgate aignet
+                                                    aigernums)))))
+    :hints((acl2::just-induct-and-expand
+            (aignet-aiger-number-nodes-iter
+             n nextgate aignet
+             aigernums)))
+    :rule-classes :linear)
+
+  ;; (defun aignet-aiger-number-nodes (aignet aigernums)
+  ;;   (declare (xargs :stobjs (aignet aigernums)
+  ;;                   :guard (and (aignet-well-formedp aignet)
+  ;;                               (u32arr-sizedp aigernums aignet))))
+  ;;   (aignet-aiger-number-nodes-iter
+  ;;    0
+  ;;    (+ 1 (lnfix (num-ins aignet)))
+  ;;    (+ 1 (lnfix (num-ins aignet)) (lnfix (num-regs aignet)))
+  ;;    aignet aigernums))
+
+
+  (defthm aigernums-size-of-aignet-aiger-number-nodes
+    (implies (< (node-count aignet) (len aigernums))
+             (< (node-count aignet) (len (aignet-aiger-number-nodes aignet aigernums))))
+    :rule-classes :linear)
+
+  (defthm aignet-number-nodes-iter-nextgate-incr
+    (implies (natp nextgate)
+             (<= nextgate
+                 (mv-nth 1 (aignet-aiger-number-nodes-iter
+                            n nextgate aignet aigernums))))
+    :hints((acl2::just-induct-and-expand
+            (aignet-aiger-number-nodes-iter
+                            n nextgate aignet aigernums)))
+    :rule-classes :linear))
+
+
+(local (defthm equal-1-when-bitp
+         (implies (and (not (equal x 0))
+                       (acl2::bitp x))
+                  (equal (equal x 1) t))
+         :hints(("Goal" :in-theory (enable acl2::bitp)))
+         :rule-classes ((:rewrite :backchain-limit-lst (0 nil)))))
+
+(definline aignet-to-aiger-lit (lit aigernums)
+  (declare (type (integer 0 *) lit)
+           (xargs :stobjs aigernums
+                  :guard (and (litp lit)
+                              (< (lit-id lit)
+                                 (u32-length aigernums)))))
+  (mk-lit
+   (get-u32 (lit-id lit) aigernums)
+   (lit-neg lit)))
+
+
+(define aiger-fanins-precede-gates (n aignet aigernums)
+  (declare (type (integer 0 *) n)
+           (xargs :guard (and (<= n (num-nodes aignet))
+                              (<= (num-nodes aignet) (u32-length aigernums)))
+                  :guard-hints (("goal" :in-theory (enable aignet-idp)))))
+  (b* (((when (zp n)) t)
+       (n (1- n))
+       ((unless (int= (id->type n aignet) (gate-type)))
+        (aiger-fanins-precede-gates n aignet aigernums))
+       (idv0 (get-u32 (lit-id (gate-id->fanin0 n aignet)) aigernums))
+       (idv1 (get-u32 (lit-id (gate-id->fanin1 n aignet)) aigernums))
+       (idvn (get-u32 n aigernums)))
+    (and (< idv0 idvn)
+         (< idv1 idvn)
+         (aiger-fanins-precede-gates n aignet aigernums)))
+  ///
+  (defcong nat-equiv equal (aiger-fanins-precede-gates n aignet aigernums) 1)
+
+
+  (defthm aiger-fanins-precede-gates-of-update-later
+    (implies (and (aiger-fanins-precede-gates
+                   n aignet aigernums)
+                  (<= (nfix n) (nfix m))
+                  (aignet-idp m aignet)
+                  ;;(<= (nfix n) (num-nodes aignet))
+                  )
+             (aiger-fanins-precede-gates
+              n aignet (update-nth m v aigernums)))
+    :hints(("Goal" :in-theory (e/d (aignet-idp)
+                                   ((:d aiger-fanins-precede-gates)))
+            :induct (aiger-fanins-precede-gates
+                     n aignet (update-nth m v aigernums))
+            :expand ((:free (aigernums)
+                      (aiger-fanins-precede-gates
+                       n aignet aigernums))
+                     (:free (aigernums)
+                      (aiger-fanins-precede-gates
+                       0 aignet aigernums)))))))
+
+(define aiger-max-id (n aignet aigernums)
+  (declare (type (integer 0 *) n)
+           (xargs :guard (and (<= n (num-nodes aignet))
+                              (<= (num-nodes aignet) (u32-length aigernums)))
+                  :verify-guards nil))
+  :returns (max natp :rule-classes :type-prescription)
+  (b* (((when (zp n)) 0)
+       (n (1- n))
+       ((when (int= (id->type n aignet) (out-type)))
+        (aiger-max-id n aignet aigernums))
+       (id (get-u32 n aigernums)))
+    (max id (aiger-max-id n aignet aigernums)))
+  ///
+  (verify-guards aiger-max-id
+    :hints (("goal" :in-theory (enable aignet-idp))))
+
+  (defcong nat-equiv equal (aiger-max-id n aignet aigernums) 1)
+
+
+  (defthm aiger-max-id-of-update-later
+    (implies (and (<= (nfix n) (nfix m))
+                  (aignet-idp m aignet))
+             (equal (aiger-max-id
+                     n aignet (update-nth m v aigernums))
+                    (aiger-max-id
+                     n aignet aigernums)))
+    :hints(("Goal" :in-theory (enable aignet-idp))))
+
+  (defthm aiger-max-id-thm
+    (implies (and (< (nfix m) (nfix n))
+                  (not (equal (id->type m aignet) (out-type))))
+             (<= (nfix (nth m aigernums))
+                 (aiger-max-id n aignet aigernums)))
+    :hints (("goal" :induct (aiger-max-id n aignet aigernums)))
+    :rule-classes nil)
+
+  (defthm aiger-max-id-of-number-nodes-iter-special
+    (b* (((mv aigernums ?nextgate)
+          (aignet-aiger-number-nodes-iter
+           n nextgate aignet aigernums)))
+      (implies (and (natp (nth m aigernums))
+                    (< (nfix m) (nfix n))
+                    (not (equal (id->type m aignet) (out-type))))
+               (<= (nth m aigernums)
+                   (aiger-max-id n aignet aigernums))))
+    :hints (("goal" :use ((:instance aiger-max-id-thm
+                           (aigernums (mv-nth 0
+                                              (aignet-aiger-number-nodes-iter
+                                               n nextgate aignet aigernums)))))))
+    :rule-classes :linear))
+
+(defthm not-out-type-when-aignet-litp
+  (implies (aignet-litp lit aignet)
+           (not (equal (ctype (stype (car (lookup-id (lit-id lit) aignet))))
+                       (out-ctype))))
+  :hints(("Goal" :in-theory (enable aignet-litp))))
+
+
+
+(defthm aiger-fanins-precede-gate-of-aignet-aiger-number-nodes-iter
+  (implies (<= (nfix n) (num-nodes aignet))
+           (b* (((mv aigernums nextgate)
+                 (aignet-aiger-number-nodes-iter
+                  n (+ 1 (stype-count (pi-stype) aignet)
+                       (stype-count (reg-stype) aignet))
+                  aignet aigernums)))
+             (and (aiger-fanins-precede-gates n aignet aigernums)
+                  (< (aiger-max-id n aignet aigernums) nextgate))))
+  :hints (("goal" :induct (aignet-aiger-number-nodes-iter
+                           n (+ 1 (stype-count (pi-stype) aignet)
+                                (stype-count (reg-stype) aignet))
+                           aignet aigernums)
+           :in-theory (e/d (aignet-idp)
+                           (aiger-fanins-precede-gates
+                            (:d aignet-aiger-number-nodes-iter)
+                            acl2::nfix-when-not-natp))
+           :expand ((:free (nextgate)
+                     (aignet-aiger-number-nodes-iter
+                      n nextgate aignet aigernums))
+                    (:free (aigernums)
+                     (aiger-fanins-precede-gates n aignet aigernums))
+                    (:free (aigernums)
+                     (aiger-max-id n aignet aigernums))
+                    (:free (aigernums)
+                     (aiger-fanins-precede-gates 0 aignet aigernums))
+                    (:free (aigernums)
+                     (aiger-max-id 0 aignet aigernums))))))
+
+(defthm aiger-fanins-precede-gate-of-aignet-aiger-number-nodes
+  (aiger-fanins-precede-gates
+   (+ 1 (node-count aignet)) aignet
+   (aignet-aiger-number-nodes aignet aigernums))
+  :hints(("Goal" :in-theory (enable aignet-aiger-number-nodes))))
+
+
+(defsection lits-ordered-when-aiger-fanins-precede-gates
+  (local (include-book "centaur/bitops/ihsext-basics" :dir :system))
+  (local (include-book "arithmetic/top-with-meta" :dir :system))
+  (defthm mk-lit-compare
+    (implies (< (nfix id1) (nfix id2))
+             (< (lit-val (mk-lit id1 neg1))
+                (lit-val (mk-lit id2 neg2))))
+    :hints(("Goal" :in-theory (e/d* (mk-lit
+                                     acl2::ihsext-redefs)))))
+
+  (defthm ids-ordered-when-aiger-fanins-precede-gates
+    (implies (and (aiger-fanins-precede-gates n aignet aigernums)
+                  (< (nfix m) (nfix n))
+                  (equal (id->type m aignet) (gate-type)))
+             (let* ((look (lookup-id m aignet))
+                    (a0 (nth (lit-id (aignet-lit-fix
+                                      (gate-node->fanin0 (car look))
+                                      (cdr look)))
+                             aigernums))
+                    (a1 (nth (lit-id (aignet-lit-fix
+                                      (gate-node->fanin1 (car look))
+                                      (cdr look)))
+                             aigernums)))
+               (and (< (nfix a0) (nfix (nth m aigernums)))
+                    ;; (implies (natp a0)
+                    ;;          (< a0 (nfix (nth m aigernums))))
+                    (< (nfix a1) (nfix (nth m aigernums)))
+                    ;; (implies (natp a1)
+                    ;;          (< a1 (nfix (nth m aigernums))))
+                    )))
+    :hints (("goal" :induct (aiger-fanins-precede-gates n aignet aigernums)
+             :in-theory (enable (:i aiger-fanins-precede-gates))
+             :expand ((aiger-fanins-precede-gates n aignet aigernums)))))
+
+  (defthm lits-ordered-when-aiger-fanins-precede-gates-1
+    (implies (and (aiger-fanins-precede-gates n aignet aigernums)
+                  (< (nfix m) (nfix n))
+                  (equal (id->type m aignet) (gate-type)))
+             (b* ((look (lookup-id m aignet))
+                  (?a0 (nth (lit-id (aignet-lit-fix
+                                     (gate-node->fanin0 (car look))
+                                     (cdr look)))
+                            aigernums))
+                  (?a1 (nth (lit-id (aignet-lit-fix
+                                     (gate-node->fanin1 (car look))
+                                     (cdr look)))
+                            aigernums))
+                  (mid (nth m aigernums)))
+               (and (< (lit-val (mk-lit a0 neg0))
+                       (lit-val (mk-lit mid 0)))
+                    (< (lit-val (mk-lit a1 neg1))
+                       (lit-val (mk-lit mid 0))))))
+    :rule-classes :linear))
+
+
+
+
+
+
+
+(defsection aignet-outs-write-aiger-lits
+  (local (defthm <-0-by-transitive
+           (implies (and (< a b)
+                         (<= 0 a))
+                    (< 0 b))
+           :rule-classes :forward-chaining))
+  (defiteration aignet-outs-write-aiger-lits (aignet aigernums channel state)
+    (declare (xargs :stobjs (aignet aigernums state)
+                    :guard (and (symbolp channel)
+                                (open-output-channel-p channel :byte state)
+                                (<= (num-nodes aignet) (u32-length aigernums)))))
+    (b* ((fanin-lit (co-id->fanin (outnum->id idx aignet) aignet))
+         (aiger-id (get-u32 (lit-id fanin-lit) aigernums))
+         (lit (mk-lit aiger-id (lit-neg fanin-lit)))
+         (state (acl2::write-ascii-nat lit channel state)))
+      (acl2::write-byte$ (char-code #\Newline) channel state))
+    :returns state
+    :index idx
+    :first 0
+    :last (num-outs aignet))
+
+  (in-theory (disable aignet-outs-write-aiger-lits))
+  (local (in-theory (enable aignet-outs-write-aiger-lits)))
+
+  (defthm open-output-channel-p1-of-aignet-outs-write-aiger-lits-iter
+    (implies (and (state-p1 state)
+                  (symbolp channel)
+                  (open-output-channel-p1 channel :byte state))
+             (let ((state (aignet-outs-write-aiger-lits-iter idx aignet aigernums channel state)))
+               (and (state-p1 state)
+                    (open-output-channel-p1 channel :byte state))))
+    :hints((acl2::just-induct-and-expand
+            (aignet-outs-write-aiger-lits-iter idx aignet aigernums channel state))))
+
+  (defthm open-output-channel-p1-of-aignet-outs-write-aiger-lits
+    (implies (and (state-p1 state)
+                  (symbolp channel)
+                  (open-output-channel-p1 channel :byte state))
+             (let ((state (aignet-outs-write-aiger-lits aignet aigernums channel state)))
+               (and (state-p1 state)
+                    (open-output-channel-p1 channel :byte state))))
+    :hints(("Goal" :in-theory (enable aignet-outs-write-aiger-lits)))))
+
+(defsection aignet-nxsts-write-aiger-lits
+  (local (defthm <-0-by-transitive
+           (implies (and (< a b)
+                         (<= 0 a))
+                    (< 0 b))
+           :rule-classes :forward-chaining))
+
+  (defiteration aignet-nxsts-write-aiger-lits (aignet aigernums channel state)
+    (declare (xargs :stobjs (aignet aigernums state)
+                    :guard (and (symbolp channel)
+                                (open-output-channel-p channel :byte state)
+                                (<= (num-nodes aignet) (u32-length aigernums)))))
+    (b* ((reg-id (regnum->id idx aignet))
+         (nxst (reg-id->nxst reg-id aignet))
+         (fanin-lit (if (int= (id->type nxst aignet) (out-type))
+                        (co-id->fanin nxst aignet)
+                      (mk-lit nxst 0)))
+         (aiger-id (get-u32 (lit-id fanin-lit) aigernums))
+         (lit (mk-lit aiger-id (lit-neg fanin-lit)))
+         (state (acl2::write-ascii-nat lit channel state)))
+      (acl2::write-byte$ (char-code #\Newline) channel state))
+    :returns state
+    :index idx
+    :first 0
+    :last (num-regs aignet))
+
+  (in-theory (disable aignet-nxsts-write-aiger-lits))
+  (local (in-theory (enable aignet-nxsts-write-aiger-lits)))
+
+  (defthm open-output-channel-p1-of-aignet-nxsts-write-aiger-lits-iter
+    (implies (and (state-p1 state)
+                  (symbolp channel)
+                  (open-output-channel-p1 channel :byte state))
+             (let ((state (aignet-nxsts-write-aiger-lits-iter idx aignet aigernums channel state)))
+               (and (state-p1 state)
+                    (open-output-channel-p1 channel :byte state))))
+    :hints((acl2::just-induct-and-expand
+            (aignet-nxsts-write-aiger-lits-iter idx aignet aigernums channel state))))
+
+  (defthm open-output-channel-p1-of-aignet-nxsts-write-aiger-lits
+    (implies (and (state-p1 state)
+                  (symbolp channel)
+                  (open-output-channel-p1 channel :byte state))
+             (let ((state (aignet-nxsts-write-aiger-lits aignet aigernums channel state)))
+               (and (state-p1 state)
+                    (open-output-channel-p1 channel :byte state))))
+    :hints(("Goal" :in-theory (enable aignet-nxsts-write-aiger-lits)))))
+
+(defsection aignet-write-aiger-gates
+  (local (in-theory (disable gate-fanin0-aignet-litp-when-aignet-nodes-ok
+                             gate-fanin1-aignet-litp-when-aignet-nodes-ok)))
+  (defiteration aignet-write-aiger-gates (aignet aigernums channel state)
+    (declare (xargs :stobjs (aignet aigernums state)
+                    :guard (and (symbolp channel)
+                                (open-output-channel-p channel :byte state)
+                                (<= (num-nodes aignet) (u32-length aigernums))
+                                (aiger-fanins-precede-gates
+                                 (num-nodes aignet) aignet aigernums))
+                    :guard-hints ('(:in-theory (enable aignet-idp)))))
+    (b* ((slot0 (id->slot id 0 aignet))
+         (type (snode->type slot0))
+         ((unless (int= type (gate-type)))
+          state)
+         (lit1 (gate-id->fanin0 id aignet))
+         (lit2 (gate-id->fanin1 id aignet))
+         (lit1 (aignet-to-aiger-lit lit1 aigernums))
+         (lit2 (aignet-to-aiger-lit lit2 aigernums))
+         ((mv lit1 lit2)
+          (if (< (lit-val lit1) (lit-val lit2))
+              (mv lit2 lit1)
+            (mv lit1 lit2)))
+         (lhslit (aignet-to-aiger-lit (mk-lit id 0) aigernums))
+         (delta1 (- (lit-val lhslit) (lit-val lit1)))
+         (delta2 (- (lit-val lit1) (lit-val lit2)))
+         (state (acl2::aiger-write-delta delta1 channel state)))
+      (acl2::aiger-write-delta delta2 channel state))
+    :returns state
+    :index id
+    :first 0
+    :last (num-nodes aignet))
+
+  (in-theory (disable aignet-write-aiger-gates))
+  (local (in-theory (enable aignet-write-aiger-gates)))
+
+  (defthm open-output-channel-p1-of-aignet-gates-write-aiger-gates-iter
+    (implies (and (state-p1 state)
+                  (symbolp channel)
+                  (open-output-channel-p1 channel :byte state))
+             (let ((state (aignet-write-aiger-gates-iter id aignet aigernums channel state)))
+               (and (state-p1 state)
+                    (open-output-channel-p1 channel :byte state))))
+    :hints((acl2::just-induct-and-expand
+            (aignet-write-aiger-gates-iter id aignet aigernums channel state))
+           '(:in-theory (disable acl2::aiger-write-delta))))
+
+  (defthm open-output-channel-p1-of-aignet-gates-write-aiger-gates
+    (implies (and (state-p1 state)
+                  (symbolp channel)
+                  (open-output-channel-p1 channel :byte state))
+             (let ((state (aignet-write-aiger-gates aignet aigernums channel state)))
+               (and (state-p1 state)
+                    (open-output-channel-p1 channel :byte state))))))
+
+
+(define aignet-write-aiger-chan (aignet (channel symbolp) state)
+  :guard (open-output-channel-p channel :byte state)
+  (b* (((local-stobjs aigernums)
+        (mv aigernums state))
+       (aigernums (resize-u32 (num-nodes aignet) aigernums))
+       (nlatches (num-regs aignet))
+       (nouts    (num-outs aignet))
+       (nins     (num-ins aignet))
+       (ngates   (num-gates aignet))
+       (aigernums (aignet-aiger-number-nodes aignet aigernums))
+       (state (acl2::aiger-write-header
+               (+ (num-ins aignet) (num-regs aignet) (num-gates aignet))
+               nins nlatches nouts ngates 0 0 channel state))
+       (state (aignet-nxsts-write-aiger-lits aignet aigernums channel state))
+       (state (aignet-outs-write-aiger-lits aignet aigernums channel state))
+       (state (aignet-write-aiger-gates aignet aigernums channel state)))
+    (mv aigernums state))
+  ///
+
+  (defthm open-output-channel-p1-of-aignet-write-aiger-chan
+    (implies (and (state-p1 state)
+                  (symbolp channel)
+                  (open-output-channel-p1 channel :byte state))
+             (let ((state (aignet-write-aiger-chan aignet channel state)))
+               (and (state-p1 state)
+                    (open-output-channel-p1 channel :byte state))))))
+
+(defttag aignet-write-aiger)
+
+(define aignet-write-aiger ((fname stringp) aignet state)
+  (b* (((mv channel state)
+        (open-output-channel! fname :byte state))
+       ((unless channel)
+        (er hard? 'aignet-write-aiger
+            "Failed to open aiger output file ~x0~%" fname)
+        state)
+       (state (aignet-write-aiger-chan aignet channel state)))
+    (close-output-channel channel state)))
+
+(acl2::defmacfun
+ aiger-write (fname &optional latch-aigs out-aigs acl2::&auto state)
+ (declare (xargs :stobjs state
+                 :guard (and (stringp fname)
+                             (true-listp latch-aigs)
+                             (true-listp out-aigs)
+                             (non-bool-atom-listp (alist-keys latch-aigs)))
+                 :guard-debug t))
+ ; (declare (xargs :mode :program))
+ (b* (((local-stobjs aignet) (mv pis state aignet))
+      (len (+ (len latch-aigs) (len out-aigs)))
+      ((mv aignet ?varmap invars ?regvars)
+       (aig-fsm-to-aignet latch-aigs out-aigs (+ 1 (* 5 len)) 2 aignet))
+      (state (aignet-write-aiger fname aignet state)))
+   (mv invars state aignet)))
+
+
+;; (defun aignet-no-outsp (n aignet)
+;;   (declare (type (integer 0 *) n)
+;;            (xargs :stobjs aignet
+;;                   :guard (and (aignet-well-formedp aignet)
+;;                               (aignet-iterator-p n aignet))))
+;;   (if (zp n)
+;;       t
+;;     (and (not (equal (id->type (to-id (1- n)) aignet) (out-type)))
+;;          (aignet-no-outsp (1- n) aignet))))
+
+;; (defcong nat-equiv equal (aignet-no-outsp n aignet) 1)
+
+;; (defun aignet-ris-unconnected (n aignet)
+;;   (declare (type (integer 0 *) n)
+;;            (xargs :stobjs aignet
+;;                   :guard (and (aignet-well-formedp aignet)
+;;                               (<= n (num-regs aignet)))
+;;                   :measure (nfix (- (nfix (num-regs aignet)) (nfix n)))))
+;;   (if (mbe :logic (zp (- (nfix (num-regs aignet)) (nfix n)))
+;;            :exec (= n (num-regs aignet)))
+;;       t
+;;     (and (int= (id->type (regnum->id n aignet) aignet) (in-type))
+;;          (aignet-ris-unconnected (+ 1 (lnfix n)) aignet))))
+
+
+(define aignet-make-n-inputs (n aignet)
+  (declare (type (integer 0 *) n))
+  (b* (((when (zp n)) aignet)
+       (aignet (aignet-add-in aignet)))
+    (aignet-make-n-inputs (1- n) aignet))
+  ///
+  (def-aignet-preservation-thms aignet-make-n-inputs)
+
+  (defthm num-inputs-of-aignet-make-n-inputs
+    (equal (stype-count (pi-stype)
+                        (aignet-make-n-inputs n aignet))
+           (+ (nfix n) (stype-count (pi-stype) aignet))))
+  
+  (defthm stype-counts-preserved-of-aignet-make-n-inputs
+    (implies (not (equal (stype-fix stype) (pi-stype)))
+             (equal (stype-count stype (aignet-make-n-inputs n aignet))
+                    (stype-count stype aignet)))))
+
+
+;; (defthm aignet-no-outsp-add-in-preserved
+;;   (implies (and (aignet-no-outsp n aignet)
+;;                 (<= (nfix n) (nfix (num-nodes aignet))))
+;;            (aignet-no-outsp n (mv-nth 1 (aignet-add-in aignet)))))
+
+;; (defthm aignet-no-outsp-of-make-n-inputs
+;;   (implies (aignet-no-outsp (nth *num-nodes* aignet) aignet)
+;;            (let ((aignet (aignet-make-n-inputs n aignet)))
+;;              (implies (equal (nfix k) (nfix (num-nodes aignet)))
+;;                       (aignet-no-outsp k aignet)))))
+
+;; (defthm aignet-ris-unconnected-add-in-preserved
+;;   (implies (and (aignet-well-formedp aignet)
+;;                 (aignet-ris-unconnected n aignet))
+;;            (aignet-ris-unconnected n (mv-nth 1 (aignet-add-in aignet))))
+;;   :hints(("Goal" :in-theory (enable* aignet-frame-thms))))
+
+;; (defthm aignet-ris-unconnected-of-make-n-inputs
+;;   (implies (and (aignet-ris-unconnected k aignet)
+;;                 (aignet-well-formedp aignet))
+;;            (let ((aignet (aignet-make-n-inputs n aignet)))
+;;              (aignet-ris-unconnected k aignet)))
+;;   :hints(("Goal" :in-theory (enable* aignet-frame-thms))))
+
+(define aignet-make-n-regs (n aignet)
+  (declare (type (integer 0 *) n))
+  (b* (((when (zp n)) aignet)
+       (aignet (aignet-add-reg aignet)))
+    (aignet-make-n-regs (1- n) aignet))
+  ///
+  (def-aignet-preservation-thms aignet-make-n-regs)
+
+  (defthm num-regs-of-aignet-make-n-regs
+    (equal (stype-count (reg-stype)
+                        (aignet-make-n-regs n aignet))
+           (+ (nfix n) (stype-count (reg-stype) aignet))))
+  
+  (defthm stype-counts-preserved-of-aignet-make-n-regs
+    (implies (not (equal (stype-fix stype) (reg-stype)))
+             (equal (stype-count stype (aignet-make-n-regs n aignet))
+                    (stype-count stype aignet)))))
+
+
+;; (defthm aignet-no-outsp-add-reg-preserved
+;;   (implies (and (aignet-no-outsp n aignet)
+;;                 (<= (nfix n) (nfix (num-nodes aignet))))
+;;            (aignet-no-outsp n (mv-nth 1 (aignet-add-reg aignet)))))
+
+;; (defthm aignet-no-outsp-of-make-n-regs
+;;   (implies (aignet-no-outsp (nth *num-nodes* aignet) aignet)
+;;            (let ((aignet (aignet-make-n-regs n aignet)))
+;;              (implies (equal (nfix k) (nfix (num-nodes aignet)))
+;;                       (aignet-no-outsp k aignet)))))
+
+;; (defthm aignet-ris-unconnected-add-reg-preserved
+;;   (implies (and (aignet-well-formedp aignet)
+;;                 (aignet-ris-unconnected n aignet))
+;;            (aignet-ris-unconnected n (mv-nth 1 (aignet-add-reg aignet))))
+;;   :hints(("Goal" :in-theory (enable* aignet-add-reg
+;;                                      aignet-frame-thms
+;;                                      nth-node-of-update-nth-node-split))))
+
+;; (defthm aignet-regnum->id-of-aignet-add-reg-prev
+;;   (implies (and (aignet-well-formedp aignet)
+;;                 (< (nfix k) (nfix (num-regs aignet))))
+;;            (equal (nth-id k (nth *regsi* (mv-nth 1 (aignet-add-reg aignet))))
+;;                   (nth-id k (nth *regsi* aignet))))
+;;   :hints(("Goal" :in-theory (enable* aignet-add-reg
+;;                                      aignet-frame-thms
+;;                                      maybe-grow-regs
+;;                                      nth-id update-nth-id))))
+
+;; (defthm num-regs-of-aignet-add-reg
+;;   (equal (nth *num-regs* (mv-nth 1 (aignet-add-reg aignet)))
+;;          (+ 1 (nfix (nth *num-regs* aignet))))
+;;   :hints(("Goal" :in-theory (enable* aignet-frame-thms
+;;                                      aignet-add-reg))))
+
+;; (defthm new-reg-of-aignet-add-reg
+;;   (implies (equal (nfix k) (nfix (num-regs aignet)))
+;;            (equal (nth-id k (nth *regsi* (mv-nth 1 (aignet-add-reg aignet))))
+;;                   (to-id (nth *num-nodes* aignet))))
+;;   :hints(("Goal" :in-theory (enable* aignet-frame-thms
+;;                                      aignet-add-reg))))
+
+;; (defthm aignet-regnum->id-of-make-n-regs-prev
+;;   (implies (and (aignet-well-formedp aignet)
+;;                 (< (nfix k) (nfix (num-regs aignet))))
+;;            (equal (nth-id k (nth *regsi* (aignet-make-n-regs n aignet)))
+;;                   (nth-id k (nth *regsi* aignet))))
+;;   :hints(("Goal" :in-theory (enable* aignet-frame-thms))))
+
+;; (defthm reg-node->ri-of-new-reg-aignet-make-n-regs
+;;   (implies (and (aignet-well-formedp aignet)
+;;                 (<= (nfix (num-regs aignet)) (nfix k))
+;;                 (< (nfix k) (nfix (num-regs (aignet-make-n-regs n aignet)))))
+;;            (equal (node->type (nth-node (nth-id k (nth *regsi* (aignet-make-n-regs n aignet)))
+;;                                       (nth *nodesi* (aignet-make-n-regs n aignet))))
+;;                   (in-type))))
+
+;; (defthm aignet-ris-unconnected-of-make-n-regs
+;;   (implies (and (aignet-ris-unconnected k aignet)
+;;                 (aignet-well-formedp aignet))
+;;            (let ((aignet (aignet-make-n-regs n aignet)))
+;;              (aignet-ris-unconnected k aignet)))
+;;   :hints (("goal" :induct t)
+;;           (and stable-under-simplificationp
+;;                '(:cases ((<= (nfix (num-regs aignet)) (nfix k)))))))
+
+;; (defthm num-regs-of-aignet-make-n-regs
+;;   (implies (natp (nth *num-regs* aignet))
+;;            (equal (nth *num-regs* (aignet-make-n-regs n aignet))
+;;                   (+ (nth *num-regs* aignet) (nfix n)))))
+
+(defstobj-clone regarr litarr :suffix "-REGS")
+(defstobj-clone outarr litarr :suffix "-OUTS")
+
+(define aignet-read-aiger-latches/outs (idx litarr ncount nxtbyte channel state)
+  (declare (type (integer 0 *) idx)
+           (type (integer 0 *) ncount)
+           (Xargs :stobjs (litarr state)
+                  :guard (and (symbolp channel)
+                              (open-input-channel-p channel :byte state)
+                              (acl2::maybe-byte-p nxtbyte)
+                              (<= ncount (lits-length litarr))
+                              (<= idx ncount))
+                  :measure (nfix (- (nfix ncount)
+                                    (nfix idx)))))
+  (b* (((when (mbe :logic (zp (- (nfix ncount)
+                                 (nfix idx)))
+                   :exec (= idx ncount)))
+        (mv nil litarr nxtbyte state))
+       ((mv num nxtbyte state)
+        (acl2::read-ascii-nat channel nxtbyte state))
+       ((when (not num))
+        (cw "Failed to parse number~%")
+        (break$)
+        (mv "Failed to parse number" litarr nxtbyte state))
+       (litarr (set-lit idx (to-lit num) litarr))
+       ((mv nxt nxtbyte state)
+        (acl2::read-byte-buf channel nxtbyte state))
+       ((when (not (eql nxt (char-code #\Newline))))
+        (cw "No newline~%")
+        (break$)
+        (mv "No newline" litarr nxtbyte state)))
+    (aignet-read-aiger-latches/outs (1+ (lnfix idx)) litarr ncount nxtbyte
+                                    channel state))
+  ///
+  (defthm lits-length-of-aignet-read-aiger-latches/outs
+    (<= (len litarr)
+        (len (mv-nth 1 (aignet-read-aiger-latches/outs
+                        idx litarr ncount nxtbyte channel
+                        state))))
+    :rule-classes :linear)
+
+  (defthm open-input-channel-p1-of-aignet-read-aiger-latches/outs
+    (implies (and (state-p1 state)
+                  (symbolp channel)
+                  (open-input-channel-p1 channel :byte state))
+             (let ((state (mv-nth 3 (aignet-read-aiger-latches/outs
+                                     idx litarr ncount nxtbyte channel state))))
+               (and (state-p1 state)
+                    (open-input-channel-p1 channel :byte state)))))
+
+  (defthm maybe-byte-p-of-aignet-read-aiger-latches/outs
+    (implies (acl2::maybe-byte-p nxtbyte)
+             (acl2::maybe-byte-p (mv-nth 2 (aignet-read-aiger-latches/outs
+                                            idx litarr ncount nxtbyte channel state))))))
+
+
+
+(local
+ (encapsulate nil
+   (local
+    (progn
+      (include-book "arithmetic/top-with-meta" :dir :system)
+
+      (defthm floor-1
+        (implies (natp x)
+                 (equal (floor x 1) x)))
+
+      (defthm niq-lte-quotient
+        (implies (and (natp a) (posp b))
+                 (<= (nonnegative-integer-quotient a b) (/ a b)))
+        :rule-classes nil)
+
+      (defthm floor-1-less
+        (implies (and (natp a)
+                      (rationalp b)
+                      (< b a))
+                 (< (floor b 1) a))
+        :hints ((and stable-under-simplificationp
+                     '(:use ((:instance niq-lte-quotient
+                              (a (numerator b)) (b (denominator b))))))))))
+
+   (defthm id-in-bounds-of-diff
+     (implies (and (posp num-nodes)
+                   (posp delta1))
+              (<
+               (LIT-ID
+                (TO-LIT
+                 (+ (LIT-VAL (MK-LIT num-nodes 0))
+                    (- delta1))))
+               num-nodes))
+     :hints(("Goal" :in-theory (e/d (lit-id mk-lit
+                                            nfix)
+                                    (floor))))
+     :rule-classes :linear)
+
+   (defthm id-in-bounds-of-diff2
+     (implies (and (posp num-nodes)
+                   (posp delta1)
+                   (natp delta2))
+              (<
+               (LIT-ID
+                (TO-LIT
+                 (+
+                  (LIT-VAL (MK-LIT num-nodes 0))
+                  (- delta1)
+                  (- delta2))))
+               num-nodes))
+     :hints (("goal" :use ((:instance id-in-bounds-of-diff
+                            (delta1 (+ delta1 delta2))))))
+     :rule-classes :linear)))
+
+(defthm aignet-not-output-when-no-outs
+  (implies (and (equal (stype-count (po-stype) aignet) 0)
+                (equal (stype-count (nxst-stype) aignet) 0))
+           (not (equal (ctype (stype (car (lookup-id id aignet))))
+                       (out-ctype))))
+  :hints(("Goal" :in-theory (enable lookup-id stype-count)
+          :induct t)
+         (and stable-under-simplificationp
+              '(:cases ((equal 1 (regp (stype (car aignet)))))))))
+
+
+;; (defthm aignet-no-outsp-of-aignet-add-gate
+;;   (implies (and (aignet-no-outsp n aignet)
+;;                 (<= (nfix n) (nfix (num-nodes aignet))))
+;;            (aignet-no-outsp n (mv-nth 1 (aignet-add-gate f0 f1 aignet)))))
+
+(define aignet-read-aiger-gates (idx numgates aignet nxtbyte channel state)
+  (declare (Xargs :stobjs (aignet state)
+                  :guard (and (symbolp channel)
+                              (open-input-channel-p channel :byte state)
+                              (acl2::maybe-byte-p nxtbyte)
+                              (natp idx) (natp numgates)
+                              (<= idx numgates)
+                              (eql (num-outs aignet) 0)
+                              (eql (num-nxsts aignet) 0))
+                  :measure (nfix (- (nfix numgates)
+                                    (nfix idx)))
+                  :guard-hints (("goal" :do-not-induct t
+                                 :in-theory (enable aignet-litp aignet-idp)))))
+  :returns (mv msg aignet nxtbyte state)
+  (b* (((when (mbe :logic (zp (- (nfix numgates)
+                                 (nfix idx)))
+                   :exec (= idx numgates)))
+        (mv nil aignet nxtbyte state))
+       (aiger-idx (lit-val (mk-lit (num-nodes aignet) 0)))
+       ((mv err delta1 nxtbyte state)
+        (acl2::read-bytecoded-nat channel nxtbyte state))
+       ((when err) (mv err aignet nxtbyte state))
+       ((when (< aiger-idx delta1))
+        (mv "Bad delta1: greater than current index"
+            aignet nxtbyte state))
+       ((when (>= 0 delta1))
+        (mv "Bad delta1: zero" aignet nxtbyte state))
+       ((mv err delta2 nxtbyte state)
+        (acl2::read-bytecoded-nat channel nxtbyte state))
+       ((when (< aiger-idx (+ delta1 delta2)))
+        (mv "Bad delta2: greater than current index - delta1"
+            aignet nxtbyte state))
+       ((when err) (mv err aignet nxtbyte state))
+       (aiger-rhs1 (- aiger-idx delta1))
+       (aiger-rhs2 (- aiger-rhs1 delta2))
+       (rhs1 (to-lit aiger-rhs1))
+       (rhs2 (to-lit aiger-rhs2))
+       (aignet (aignet-add-gate rhs1 rhs2 aignet)))
+    (aignet-read-aiger-gates
+     (1+ (nfix idx)) numgates aignet nxtbyte channel state))
+
+  ///
+
+  (defthm open-input-channel-p1-of-aignet-read-aiger-gates
+    (implies (and (state-p1 state)
+                  (symbolp channel)
+                  (open-input-channel-p1 channel :byte state))
+             (let ((state (mv-nth 3 (aignet-read-aiger-gates
+                                     idx numgates aignet nxtbyte channel state))))
+               (and (state-p1 state)
+                    (open-input-channel-p1 channel :byte state)))))
+
+  (defthm maybe-byte-p-of-aignet-read-aiger-gates
+    (implies (acl2::maybe-byte-p nxtbyte)
+             (acl2::maybe-byte-p (mv-nth 2 (aignet-read-aiger-gates
+                                            idx numgates aignet nxtbyte channel
+                                            state)))))
+
+  (def-aignet-preservation-thms aignet-read-aiger-gates)
+
+  (defthm stype-counts-preserved-of-aignet-read-aiger-gates
+    (implies (not (equal (stype-fix stype) (gate-stype)))
+             (equal (stype-count stype (mv-nth 1 (aignet-read-aiger-gates
+                                                  idx numgates aignet nxtbyte
+                                                  channel state)))
+                    (stype-count stype aignet)))))
+
+
+;; (def-aignet-frame aignet-read-aiger-gates
+;;   :hints (("goal" :induct (aignet-read-aiger-gates
+;;                            idx numgates aignet nxtbyte channel state)
+;;            :in-theory (disable (:definition aignet-read-aiger-gates))
+;;            :expand ((aignet-read-aiger-gates idx numgates aignet nxtbyte channel
+;;                                              state))
+;;            :do-not-induct t)))
+
+;; (def-aignet-preservation-thms aignet-read-aiger-gates)
+
+;; (defthm num-nodes-of-aignet-read-aiger-gates
+;;   (implies (natp (nth *num-nodes* aignet))
+;;            (<= (nth *num-nodes* aignet)
+;;                (nth *num-nodes* (mv-nth 1 (aignet-read-aiger-gates
+;;                                           idx numgates aignet nxtbyte channel
+;;                                           state)))))
+;;   :rule-classes (:rewrite :linear))
+
+;; (defthm aignet-ris-unconnected-of-aignet-read-aiger-gates
+;;   (implies (and (aignet-ris-unconnected k aignet)
+;;                 (aignet-well-formedp aignet))
+;;            (let ((aignet (mv-nth 1 (aignet-read-aiger-gates idx numgates aignet
+;;                                                          nxtbyte channel state))))
+;;              (aignet-ris-unconnected k aignet)))
+;;   :hints (("goal" :induct t
+;;            :in-theory (enable* aignet-frame-thms))))
+
+;; (defthm aignet-ris-unconnected-of-aignet-add-regin
+;;   (implies (and (aignet-ris-unconnected k aignet)
+;;                 (aignet-idp (id-fix ro) aignet)
+;;                 (< (io-id->ionum ro aignet) (nfix k))
+;;                 (aignet-well-formedp aignet))
+;;            (aignet-ris-unconnected k (aignet-add-regin f ro aignet)))
+;;   :hints(("Goal" :in-theory (enable* aignet-frame-thms
+;;                                      aignet-idp)
+;;           :induct t)
+;;          (and stable-under-simplificationp
+;;               '(:use ((:instance aignet-well-formedp-regnum
+;;                        (n k)))
+;;                 :in-theory (e/d* (aignet-add-regin
+;;                                   aignet-add-regin1
+;;                                   aignet-idp
+;;                                   aignet-unconnected-reg-fixup
+;;                                   aignet-frame-thms)
+;;                                  (aignet-well-formedp-regnum))))))
+
+;; (defthm aignet-no-outsp-of-aignet-read-aiger-gates
+;;   (implies (aignet-no-outsp (nth *num-nodes* aignet) aignet)
+;;            (let ((aignet (mv-nth 1 (aignet-read-aiger-gates idx numgates aignet nxtbyte channel
+;;                                                          state))))
+;;              (implies (equal (nfix k) (nfix (num-nodes aignet)))
+;;                       (aignet-no-outsp k aignet))))
+;;   :hints(("goal" :induct t
+;;           :expand ((aignet-no-outsp k aignet)))))
+
+;; (defthm aignet-no-outsp-of-aignet-add-regin
+;;   (implies (and (aignet-no-outsp k aignet)
+;;                 (<= (nfix k) (nfix (num-nodes aignet))))
+;;            (aignet-no-outsp k (aignet-add-regin f ro aignet)))
+;;   :hints(("Goal" :in-theory (enable* aignet-frame-thms))))
+
+
+(local
+ (defthm aignet-not-output-when-no-outs2
+   (implies (and (equal (stype-count (po-stype) aignet2) 0)
+                 (equal (stype-count (nxst-stype) aignet2) 0)
+                 (<= (nfix id) (node-count aignet2))
+                 (aignet-extension-p aignet aignet2))
+            (not (equal (ctype (stype (car (lookup-id id aignet))))
+                        (out-ctype))))
+   :hints(("Goal" :in-theory (enable lookup-id stype-count aignet-extension-p)
+           :induct t)
+          (and stable-under-simplificationp
+               '(:cases ((equal 1 (regp (stype (car aignet))))))))))
+
+(define aignet-aiger-copy-nxsts (idx maxid regarr aignet)
+  (declare (type (integer 0 *) idx)
+           (type (integer 1 *) maxid)
+           (xargs :stobjs (regarr aignet)
+                  :guard (and (<= (num-regs aignet) (lits-length regarr))
+                              (<= idx (num-regs aignet))
+                              (<= maxid (num-nodes aignet))
+                              (non-exec
+                               (and (equal (num-outs (lookup-id (1- maxid) aignet))
+                                           0)
+                                    (equal (num-nxsts (lookup-id (1- maxid) aignet))
+                                           0))))
+                  :measure (nfix (- (nfix (num-regs aignet))
+                                    (nfix idx)))
+                  :guard-hints(("goal" 
+                                :in-theory (enable* aignet-litp aignet-idp)
+                                :do-not-induct t))))
+  :guard-debug t
+  (b* (((when (mbe :logic (zp (- (nfix (num-regs aignet))
+                                    (nfix idx)))
+                   :exec (int= idx (num-regs aignet))))
+        (mv nil aignet))
+       (fanin (get-lit idx regarr))
+       ((when (<= (lnfix maxid) (lit-id fanin)))
+        (mv "PO fanin out of bounds" aignet))
+       (ro (regnum->id idx aignet))
+       (aignet (aignet-set-nxst fanin ro aignet)))
+    (aignet-aiger-copy-nxsts (1+ (lnfix idx)) maxid regarr aignet))
+
+  ///
+  (def-aignet-preservation-thms aignet-aiger-copy-nxsts)
+
+  (defthm stype-counts-preserved-of-aignet-aiger-copy-nxsts
+    (implies (not (equal (stype-fix stype) (nxst-stype)))
+             (equal (stype-count stype (mv-nth 1 (aignet-aiger-copy-nxsts
+                                                  idx maxid regarr aignet)))
+                    (stype-count stype aignet)))))
+
+  
+
+;; (local (defthm linear-help1
+;;          (implies (and (< (id-val (lit-id bla-bla)) maxid)
+;;                        (<= maxid (nth *num-nodes* aignet)))
+;;                   (< (id-val (lit-id bla-bla)) (nth *num-nodes* aignet)))))
+
+
+;; (local (in-theory (disable linear-help1)))
+
+;; (defthm aignet-no-outsp-of-aignet-add-out
+;;   (implies (and (aignet-no-outsp k aignet)
+;;                 (<= (nfix k) (nfix (num-nodes aignet))))
+;;            (aignet-no-outsp k (aignet-add-out f aignet)))
+;;   :hints(("Goal" :in-theory (enable* aignet-frame-thms))))
+
+(define aignet-aiger-copy-outs (idx maxid outarr outnum aignet)
+  (declare (type (integer 0 *) idx)
+           (type (integer 1 *) maxid)
+           (type (integer 0 *) outnum)
+           (xargs :stobjs (outarr aignet)
+                  :guard (and (<= outnum (lits-length outarr))
+                              (<= maxid (num-nodes aignet))
+                              (<= idx outnum)
+                              (non-exec
+                               (and (equal (num-outs (lookup-id (1- maxid) aignet))
+                                           0)
+                                    (equal (num-nxsts (lookup-id (1- maxid) aignet))
+                                           0))))
+                  :measure (nfix (- (nfix outnum)
+                                    (nfix idx)))
+                  :guard-hints(("goal" 
+                                :in-theory (enable* aignet-idp aignet-litp)
+                                :do-not-induct t))))
+  (b* (((when (mbe :logic (zp (- (nfix outnum)
+                                 (nfix idx)))
+                   :exec (int= idx outnum)))
+        (mv nil aignet))
+       (fanin (to-lit (get-lit idx outarr)))
+       ((when (<= (lnfix maxid) (lit-id fanin)))
+        (mv "Register fanin out of bounds" aignet))
+       (aignet (aignet-add-out fanin aignet)))
+    (aignet-aiger-copy-outs (1+ (lnfix idx)) maxid outarr outnum aignet))
+  ///
+
+  (def-aignet-preservation-thms aignet-aiger-copy-outs)
+
+  (defthm stype-counts-preserved-of-aignet-aiger-copy-outs
+    (implies (not (equal (stype-fix stype) (po-stype)))
+             (equal (stype-count stype (mv-nth 1 (aignet-aiger-copy-outs
+                                                  idx maxid outarr outnum aignet)))
+                    (stype-count stype aignet)))))
+
+(local
+ (defthm natp-nth-in-nat-list
+   (implies (and (nat-listp x)
+                 (natp n)
+                 (< n (len x)))
+            (natp (nth n x)))
+   :hints(("Goal" :in-theory (enable nth)))
+   :rule-classes (:rewrite :type-prescription)))
+
+
+(local (in-theory (disable acl2::aiger-parse-header
+                           acl2::make-list-ac-redef
+                           make-list-ac)))
+
+;; The functions we're using from aiger.lisp take a "buf", which is really just
+;; either the next byte of the file or else NIL, so that they can do lookahead.
+(define aignet-read-aiger-chan (aignet channel state)
+  (declare (xargs :guard (and (symbolp channel)
+                              (open-input-channel-p channel :byte state))
+                  :guard-debug t
+                  :guard-hints (("goal"
+                                 :do-not-induct t))))
+  (b* (((mv err i l a o b c nxtbyte state)
+        (acl2::aiger-parse-header channel nil state))
+       ((when err) (mv err aignet state))
+       (aignet (aignet-init (+ 1 o b c) (+ 1 l) (+ 1 i) (+ 1 a l o b c) aignet))
+       ((local-stobjs outarr regarr)
+        (mv err aignet state outarr regarr))
+       (outarr (resize-lits (+ o b c) outarr))
+       (regarr (resize-lits l regarr))
+       (aignet (aignet-make-n-inputs i aignet))
+       (aignet (aignet-make-n-regs l aignet))
+       ((mv err regarr nxtbyte state)
+        (aignet-read-aiger-latches/outs 0 regarr l nxtbyte channel state))
+       ((when err) (mv err aignet state outarr regarr))
+       ((mv err outarr nxtbyte state)
+        (aignet-read-aiger-latches/outs 0 outarr (+ o b c) nxtbyte channel state))
+       ((when err) (mv err aignet state outarr regarr))
+       ((mv err aignet ?nxtbyte state)
+        (aignet-read-aiger-gates 0 a aignet nxtbyte channel state))
+       ((when err) (mv err aignet state outarr regarr))
+       (- (and (not (= (nfix (num-gates aignet)) a))
+               (er hard? 'aignet-read-aiger
+                   "Wrong number of gates read: ~x0, should be ~x1~%"
+                   (num-gates aignet) a)))
+       (maxid (num-nodes aignet))
+       ((mv err aignet) (aignet-aiger-copy-nxsts 0 maxid regarr aignet))
+       ((when err) (mv err aignet state outarr regarr))
+       ((mv err aignet) (aignet-aiger-copy-outs 0 maxid outarr (+ o b c) aignet)))
+    (mv err aignet state outarr regarr))
+
+  ///
+
+  (defthm open-input-channel-p1-of-aignet-read-aiger-chan
+    (implies (and (state-p1 state)
+                  (symbolp channel)
+                  (open-input-channel-p1 channel :byte state))
+             (let ((state (mv-nth 2 (aignet-read-aiger-chan
+                                     aignet channel state))))
+               (and (state-p1 state)
+                    (open-input-channel-p1 channel :byte state))))))
+
+(define aignet-read-aiger (fname aignet state)
+  (declare (xargs :guard (stringp fname)))
+  (b* (((mv channel state) (open-input-channel fname :byte state))
+       ((when (not channel))
+        (mv "Could not open input file" aignet state))
+       ((mv err aignet state)
+        (aignet-read-aiger-chan aignet channel state))
+       (state (close-input-channel channel state)))
+    (mv err aignet state)))
+
+
+
+ 
