books/branches/jared/centaur/ccl-config.lsp
@@ -89,3 +89,4 @@
 (save-application *heap-image-name*)
 
 (quit)
+
